\documentclass{article}

\usepackage{amsmath, amsfonts, amssymb, amsthm}
\usepackage{hyperref}

\setlength{\parindent}{0pt}
\setlength{\parskip}{5pt}

\title{IMO 2009 A5}
\author{}
\date{}

\begin{document}

\maketitle



\subsection*{Problem}

Let $F$ be a totally ordered field.
Prove that, for any function $f : F \to F$, there exists $x, y \in F$ such that $f(x - f(y)) > y f(x) - x$.



\subsection*{Solution}

Official solution: \url{https://www.imo-official.org/problems/IMO2009SL.pdf}

The following solution is a rewrite of Solution 1 of the official solution.
We modify the ordering and the wording of the solution a bit.

We proceed by contradiction.
Assume that, for all $x, y \in F$,
\[ f(x - f(y)) \leq y f(x) - x. \tag{*}\label{eq0} \]
First, plugging $(x, y) = (t + f(0), 0)$ yields that for all $t \in F$,
\[ f(t) \leq t + f(0). \tag{1}\label{eq1} \]
We now split into two cases:

\begin{itemize}

    \item 
    For all $x \in F$, $f(x) \leq 0$.

    Pick some $t \in F$ such that $t > \max\{0, -f(-1) - 1\}$.
    We claim that in fact, $f(-1) \leq -t - 1$, contradicting $t > -f(-1) - 1$.
    The fact that $f(0) \leq 0$ means that~\eqref{eq1} implies $f(x) \leq x$ for all $x \in F$.
    Then, plugging $(x, y) = (f(t) - 1, t)$ into~\eqref{eq0} now yields
    \[ f(-1) \leq tf(f(t) - 1) + f(t) - 1 \leq (t + 1)(f(t) - 1). \]
    But $f(t) \leq 0$ and $t + 1 > t > 0$, so this yields $f(-1) \leq -(t + 1) = -t - 1$.

    \item
    There exists $c \in F$ such that $f(c) > 0$.

    Pick some $t \in F$ such that $t < \min\left\{c - f(0), \dfrac{-f(0) - c - 1}{f(c)}\right\}$.
    We claim that in fact, $-f(0) - 1 \leq tf(c) + c$, contradicting $t < \dfrac{-f(0) - c - 1}{f(c)}$.
    Indeed, by~\eqref{eq0} and~\eqref{eq1}, letting $y = c - f(t)$,
    \[ tf(c) + c \geq f(y) \geq f(f(y)) - f(0). \]
    On the other hand, plugging $x = f(y)$ into~\eqref{eq0} yields
    \[ f(0) \leq y f(f(y)) + f(y) \leq y f(f(y)) + y + f(0) \implies y (f(f(y)) + 1) \geq 0. \]
    Finally, note that $y > 0$ by~\eqref{eq1}.
    Indeed, $y = c - f(t) \geq c - (t + f(0)) > 0$.
    This yields $f(f(y)) \geq -1$; a contradiction.

\end{itemize}




\end{document}
