# IMO 2007 A2

We call a function $f : \N^+ \to \N^+$ good if for any $m, n \in \N^+$,
$$ f(m + n) + 1 \geq f(m) + f(f(n)). $$
Fix some $N \in \N^+$.
Determine all $k \in \N^+$ for which there exists a good function $f$ with $f(N) = k$.



# Answer

$k \leq N + 1$ for $N > 1$, and just $k = 1$ for $N = 1$.



# Solution

Official solution: <https://www.imo-official.org/problems/IMO2007SL.pdf>

Instead of dealing directly with good functions, we analyze functions $g : \N \to \N$ satisfying $g(m + n + 1) \geq g(m) + g(g(n))$ for all $m, n \in \N$.
This is obtained by the substitution $f(n) = g(n + 1) - 1$.
The question becomes as follows: given $N \in \N$, determine all $k \in \N$ such that there exists $g : \N \to \N$ satisfying the above inequality with $g(N) = k$.
The answer is $k \leq N + 1$ for $N > 0$ and $k = 0$ for $N = 0$.

For the case $k \leq N$, the example from the official solution translates to the function $g_K(n) = \max\{0, n - K\}$ for some suitable $K \geq 0$ (in this case, $K = N - k$).
Meanwhile, for the case $k = N + 1$, the example translates to the following function with $K = N + 1$:
$$ h_K(n) = \begin{cases} n, & K \nmid n + 1, \\ n + 1, & K \mid n + 1. \end{cases} $$
Thus it remains to prove that $g(n) \leq n + 1$ for any $n \in \N$ and $g(0) = 0$.

Monotonicity is easy from $g(m + n + 1) \geq g(m) + g(g(n)) \geq g(m)$ for all $m, n \in \N$.
Indeed, for any $b \geq a$, if $b = a$ then clearly $f(b) \geq f(a)$.
If $b > a$, then plugging $m = a$ and $n = b - a - 1$ yields the result.

If $g(0) > 0$ then we have $g(1) \geq g(0) + g(g(0)) > g(g(0))$.
Since $g$ is monotone (increasing), this yields $g(0) < 1$; a contradiction.
Thus $g(0) = 0$.

Now fix some $k > 1$ and suppose for the sake of contradiction that $g(k) > k + 1$.
We can write $g(k) = k + d + 1$ for some $d > 0$.
First, for any such $k$ and $d$, plugging $m = d$ and $n = k$ yields $g(d) = 0$.
In particular, since $g(d) < g(k)$, we must have $d < k$.

Now, plugging $n = k$ yields that for all $m \in \N$,
$$ g(m + k + 1) \geq g(m) + g(k + d + 1) \geq g(m) + g(k) = g(m) + k + d + 1. $$
By small induction, for any $j \geq 0$,
$$ g(m + j(k + 1)) \geq g(m) + j(k + d + 1). $$
In particular, we get $g((k + 1)^2) \geq (k + 1)(k + d + 1) = (k + 1)^2 + (k + 1)d$.
By the previous paragraph, $(k + 1)d - 1 < k$; a contradiction since $d > 0$.
This shows that $g(k) \leq k + 1$ for all $k \in \N$.



# Implementation notes

Instead of dealing directly with good functions, we analyze functions $g : \N \to \N$ satisfying $g(m + n + 1) \geq g(m) + g(g(n))$ for all $m, n \in \N$.
It can be easily shown that $f$ is good if and only if $g = x \mapsto f(x + 1) - 1$ satisfies the above inequality.

We will present results for both versions with `pnat` and with `nat`.
