# IMO 2017 A8, Generalized Version

Let $G$ be a linear densely ordered (additive) abelian group.
Let $f : G \to G$ be a function such that, for any $x, y \in G$ with $f(x) < f(y)$, we have $f(x) \leq x + y \leq f(y)$.
Prove that $f(x) \leq f(y)$ for all $x < y$.



# Solution

Fix some $x, y \in G$ such that $x < y$ and $f(x) > f(y)$.
We nearly characterizes elements $z \in G$ such that $f(z) \in \{f(x), f(y)\}$.

> __Lemma 1__:
> For any $z \in G$, if $z < f(y) - y$, then $f(z) < f(y)$.
>
> __Proof__:
> If $f(z) > f(y)$, then $f(y) \leq y + z$ which implies $z \geq f(y) - y$; a contradiction.
> If $f(z) = f(y) < f(x)$, then $f(y) \leq z + x$, which implies $z \geq f(y) - x \geq f(y) - y$; a contradiction.

> __Lemma 2__:
> For any $z \in G$, if $z > f(x) - x$, then $f(z) > f(x)$.
>
> __Proof__:
> The proof is very similar to Lemma 3.
> If $f(z) < f(x)$, then $z + x \leq f(x)$ which implies $z \leq f(x) - x$; a contradiction.
> If $f(z) = f(x) > f(y)$, then $f(x) \geq z + y$, which implies $z \leq f(x) - y \leq f(x) - x$; a contradiction.

> __Lemma 3__:
> For any $z \in G$, if $f(y) - y < z < f(x) - x$, then $f(z) \in \{f(x), f(y)\}$.
>
> __Proof__:
> If $f(z) < f(y)$, then $y + z \leq f(y)$, so $z \leq f(y) - y$.
> If $f(z) > f(x)$, then $x + z \geq f(x)$, so $z \geq f(x) - x$.
> If $f(y) < f(z) < f(x)$, $y + z \leq f(z) \leq x + z$, so $y \leq x$.
> All the three cases contradict the lemma's assumption since $x < y$ and $f(y) - y < z < f(x) - x$.

Using the fact that $G$ is densely ordered, we now obtain a contradiction.
Pick some $z \in G$ such that $x < z < y$.
Since $f(y) \leq x + y \leq f(x)$, we have $z > x \geq f(y) - y$ and $z < y \leq f(x) - x$.
That means Lemma 3 yields either $f(z) = f(x)$ or $f(z) = f(y)$.

First, suppose that $f(z) = f(x) > f(y)$.
Pick some $w \in G$ such that $x < w < z < y$.
Then we have $f(y) - y < f(z) - z < f(x) - w < f(x) - x$.
By Lemma 3, we have $f(f(z) - w) \in \{f(x), f(y)\}$.
By Lemma 2 using $f(z) - w > f(z) - z$, we have $f(f(x) - w) > f(z) = f(x)$; a contradiction.

Now suppos that $f(z) = f(y) < f(x)$.
Pick some $w \in G$ such that $x < z < w < y$.
Then we have $f(y) - y < f(z) - w < f(z) - z < f(x) - x$.
By Lemma 3, $f(f(z) - w) \in \{f(x), f(y)\}$.
By Lemma 2 using $f(z) - w < f(z) - z$, we have $f(f(x) - w) < f(z) = f(y)$; a contradiction.



# Extra

In the original version, we are given $f : \R \to \R$ such that for any $x, y \in \R$, if $(f(x) + y)(f(y) + x) > 0$, then $f(x) + y = f(y) + x$.
While it follows from the general version, it is not a direct result on the general case by simply replacing $G$ with $\R$.
We still need a slight manipulation, so we will implement the original version (with linear ordered rings) in another file, `A8_original.lean`.

The result does not hold anymore when $G$ is not densely ordered, e.g. when $G = \Z$.
Indeed, define a function $f : \Z \to \Z$ by $f(0) = 2$, $f(1) = 0$, and $f(x) = 2x$ for $x \notin \{0, 1\}$.
For any $x, y \in \Z$ with $f(x) < f(y)$, we have several cases.
Except for the case $(x, y) = (1, 0)$, we have $x < y$.
1. If $(x, y) = (1, 0)$, then $f(1) = 0 \leq 1 + 0 \leq 2 = f(0)$.
2. If $x < 0$ and $y \in \{0, 1\}$, then $f(x) = 2x \leq x \leq x + y \leq 0 \leq f(y)$.
3. If $x \in \{0, 1\}$ and $y > 1$, then $f(x) \leq 2 \leq x + y \leq 2y = f(y)$.
4. If $x < y$ and $x, y \notin \{0, 1\}$, we have $f(x) = 2x \leq x + y \leq 2y = f(y)$.
The above cases are exhaustive, so indeed we always have $f(x) \leq x + y \leq f(y)$.
On the other hand, we have $0 < 1$ and yet $f(0) > f(1)$.
We implement this counterexample in `A8_counter.lean`.
