\documentclass{article}

\usepackage{amsmath, amsfonts, amssymb, amsthm}
\usepackage{hyperref}

\setlength{\parindent}{0pt}
\setlength{\parskip}{5pt}

\newcommand{\R}{\mathbb{R}}

\title{IMO 2006 A6 (P3)}
\author{}
\date{}

\begin{document}

\maketitle



\subsection*{Problem}

Find the smallest real number $M$ such that, for any $a, b, c \in \R$,
\[ |ab(a^2 - b^2) + bc(b^2 - c^2) + ca(c^2 - a^2)| \leq M(a^2 + b^2 + c^2)^2. \tag{*}\label{2006a6-eq0} \]



\subsection*{Answer}

$\dfrac{9}{32} \sqrt{2}$.



\subsection*{Solution}

Official solution: \url{https://www.imo-official.org/problems/IMO2006SL.pdf}

We present the official solution with shortcuts, relying on some polynomial identities to prove inequalities.
In particular, we make use of the two identities
\[ ab(a^2 - b^2) + bc(b^2 - c^2) + ca(c^2 - a^2) = (b - a)(c - b)(a - c)(a + b + c), \]
\[ (b - c)^2 + (c - a)^2 + (a - b)^2 + (a + b + c)^2 = 3(a^2 + b^2 + c^2). \]

To prove that $M \geq \frac{9}{32} \sqrt{2}$, take $a = \sqrt{2}$, $b = \sqrt{2} - 3$, and $c = \sqrt{2} + 3$.
Using the above identity, one checks that the left hand side equals $2 \cdot 3^4 \sqrt{2}$.
On the other hand, the right hand side equals $M(3 \cdot 2 + 2 \cdot 3^2)^2 = 2^6 \cdot 3^2 M$.
Thus we get $M \geq \frac{9}{32} \sqrt{2}$.

We now prove that $M = \frac{9}{32} \sqrt{2}$ works.
Let $s = a + b + c$, $x = b - a$, $y = c - b$, and $z = a - c$.
Based on the above identities,~\eqref{2006a6-eq0} becomes $16 \sqrt{2} |sxyz| \leq (s^2 + x^2 + y^2 + z^2)^2$.
Equivalently, $2^9 (sxyz)^2 \leq (s^2 + x^2 + y^2 + z^2)^4$.
We now prove this inequality, noting that $x + y + z = 0$.

Start by using AM-GM of the form $(r + 3t)^4 \geq 4^4 rt^3$ for any $r, t \in \R$.
In particular, here we get
\[ 3^4 (s^2 + x^2 + y^2 + z^2)^4 \geq 4^4 \cdot 3 s^2 (x^2 + y^2 + z^2)^3. \]
Thus it remains to prove that $2 \cdot 3^3 (xyz)^2 \leq (x^2 + y^2 + z^2)^3$.
Indeed, after substituting $z = -(x + y)$, this inequality reduces to $54 x^2 y^2 (x + y)^2 \leq 8 (x^2 + y^2 + xy)^3$.
One checks that $8 (x^2 + y^2 + xy)^3 - 54 x^2 y^2 (x + y)^2 = 2 (x - y)^2 (x + 2y)^2 (2x + y)^2$, which is obviously non-negative.
We are done.



\subsection*{Implementation details}

We prove the lower bound in a separate file: \texttt{A6\_general.lean}.
The real case is solved in the main file: \texttt{A3\_main.lean}.
The file \texttt{A3\_general.lean} does not need to import \texttt{data.real.basic} module, keeping results general.



\end{document}
