# IMO 2017 C7

For any finite set $X \subseteq \N$, denote by $f_X(k)$ the $k^{\text{th}}$ smallest natural number not in $X$, indexed from $0$.
For any finite sets $X, Y \subseteq \N$, denote $X * Y = X \cup \{f_X(y) : y \in Y\}$.
Also, for any finite set $X \subseteq \N$ and $k \geq 0$, define $X^k$ recursively by $X^0 = \emptyset$ and $X^{k + 1} = X * X^k$.

Let $A$ and $B$ be finite subsets of $\N$, and suppose that $A * B = B * A$.
Prove that $A^{|B|} = B^{|A|}$.



# Solution

Official solution: <http://www.imo-official.org/problems/IMO2017SL.pdf>

We follow Solution 1.
However, we will prove Lemma 2 in a different way.
More generally, we prove the following.

> __Lemma__:
> Let $f, g : \N \to \N$ be a strictly increasing function such that $f \circ g = g \circ f$.
> Suppose that, for some $N \in \N$, we have $f(n) = g(n)$ for all $n \geq N$.
> Then $f = g$.
>
> __Proof__:
> We proceed by downwards induction.
> Given some $k > 0$, suppose that $f(n) = g(n)$ holds for all $n > k$.
> Since $f$ and $g$ are strictly increasing, we have $f(k), g(k) \geq k$.
> If $f(k) > k$, then by induction hypothesis, $f(g(k)) = g(f(k)) = f(f(k))$.
> Strictly increasing functions are injective, so this means $f(k) = g(k)$.
> We also get $f(k) = g(k)$ for $g(k) > k$.
> The only remaining case leads to $f(k) = g(k) = k$.

To prove Lemma 2, let $X, Y \subseteq \N$ be finite subsets with $|X| = |Y|$ and $X * Y = Y * X$.
We have $f_X(s) = s + |X| = s + |Y| = f_Y(s)$ for all $s > \max(X \cup Y)$.
On the other hand, $f_X \circ f_Y = f_{X * Y} = f_{Y * X} = f_Y \circ f_X$.
Clearly, $f_X$ and $f_Y$ are strictly increasing, so the above lemma indeed gives $f_X = f_Y$ and thus $X = Y$.



# Implementation notes

The original formulation uses positive integers, for both the supersets of $X$ and $Y$ and also the indexing set.
We use non-negative integers for implementation convenience.
Also, the original formulation asks only for the case where $A$ and $B$ are non-empty.
Due to our definition, we can extend to the empty case.

It seems that our above way to prove Lemma 2 is somewhat similar to one in Solution 2.
