\documentclass{article}

\usepackage{amsmath, amsfonts, amssymb, amsthm}
\usepackage{hyperref}

\setlength{\parindent}{0pt}
\setlength{\parskip}{5pt}

\title{IMO 2014 N2}
\author{}
\date{}

\begin{document}

\maketitle



\subsection*{Problem}

Find all pairs $(x, y)$ of integers such that
\[ 7 (x^2 + y^2) - 13 xy = (|x - y| + 1)^3. \tag{*}\label{2014n2-eq0} \]



\subsection*{Answer}

$(x, y) = (A(m), B(m))$ and $(x, y) = (B(m), A(m))$ for some integer $m$.
Here $A(m) = m^3 + 2m^2 - m - 1$ and $B(m) = m^3 + m^2 - 2m - 1$.



\subsection*{Solution}

Official solution: \url{https://www.imo-official.org/problems/IMO2014SL.pdf}

We present a copy of the official solution.

First note that $7 (x^2 + y^2) - 13 xy = 7 (x - y)^2 + xy$.
To verify that the pairs given as answers satisfy~\eqref{2014n2-eq0}, first we check that $A(m) - B(m) = m(m + 1)$.
Then the equality reduces to $7(m^2 + m)^2 + 13(m^3 + 2m^2 - m - 1)(m^3 + m^2 - 2m - 1) = (m^2 + m + 1)^3$.
This can be done, for example, by brute force.

For the converse, WLOG let $x \geq y$, and write $x - y = n$.
Then~\eqref{2014n2-eq0} becomes $7n^2 + ny + y^2 = (n + 1)^3$.
By brute force, one checks that $4(ny + y^2) + n^2 = (2y + n)^2$ and $4((n + 1)^3 - 7n^2) + n^2 = (n - 2)^2 (4n + 1)$.
As a result, we have $(2n + y)^2 = (n - 2)^2 (4n + 1)$.
In particular, if $n \neq 2$, then $(2n + y) = (n - 2) k$ for some integer $k$ with $k^2 = 4n + 1$.
Otherwise, $n = 2$ yields $y = -1 = B(1)$ and $x = 1 = A(1)$.

Now, since $k^2 = 4n + 1$, we can write $k = 2m + 1$ and $n = m^2 + m$ for some integer $m$.
Finally, $2n + y = (n - 2) k$ yields $y = (n - 2) k + 2n = B(m)$ and $x = n + y = A(m)$.



\end{document}
