# IMO 2013 N6

Determine all functions $f : \mathbb{Q} \to \Z$ such that, for all $x \in \mathbb{Q}$, $a \in \Z$, and $b \in \N^+$,
$$ f\left(\frac{f(x) + a}{b}\right) = f\left(\frac{x + a}{b}\right). $$



# Answer

Constants, the floor function, and the ceiling function.



# Solution

Official solution: <https://www.imo-official.org/problems/IMO2013SL.pdf>

We will not actually follow the official solution, except for one minor step: showing that $f(1/2) \in \{0, 1\}$.
In fact, we will use a different case distinction as well.
The first case lead to $f$ being constant easier, while the second case also easily implies $f(m) = m$ for all $m \in \Z$.

Denote the original equality by $(*)$.


## Case 1: $f(0) = f(1)$.

Comparing the $(*)$ with $x = 0$ and $x = 1$, we get $f\left(\frac{a}{b}\right) = f\left(\frac{a + 1}{b}\right)$ for all $a \in \Z$ and $b \in \N^+$.
Then by induction, we get
$$ f\left(\frac{a}{b}\right) = f\left(\frac{a + n}{b}\right) $$
for all $a \in \Z$, $n \in \N$, and $b \in \N^+$.
For any rational number $x$, we can write $x = \frac{a}{b}$ for some $a \in \Z$ and $b \in \N^+$.
If $a < 0$, use $n = -a$ to get $f(x) = f(0)$.
If $a > 0$, then replace $a$ with $-a$ and use $n = a$ in the above equality to get $f(x) = f(0)$.
This means that $f$ is constant.


## Case 2: $f(0) \neq f(1)$.

First, we show that $f(m) = m$ for all $m \in \Z$.
Indeed, fix some integer $m$.
If $f(m) < m$, plugging $(x, a, b) = (m, -f(m), m - f(m))$ into $(*)$ yields $f(0) = f(1)$.
If $f(m) > m$, plugging $(x, a, b) = (m, -m, f(m) - m)$ into $(*)$ yields $f(0) = f(1)$.
Both yields a contradiction, so we have $f(m) = m$.

Next, we show that $f(1/2) \in \{0, 1\}$, following the official solution.
If $f(1/2) \leq 0$, plugging $(x, a, b) = (1/2, -f(1/2), 1 - 2f(1/2))$ into $(*)$ yields $f(1/2) = 0$.
Otherwise, we have $f(1/2) \geq 1$.
Then plugging $(x, a, b) = (1/2, 1 - f(1/2), 2f(1/2) - 1)$ into $(*)$yields $f(1/2) = 1$.

One checks that, given a function $f : \mathbb{Q} \to \Z$ satisfying $(*)$, the function $x \mapsto -f(-x)$ also satisfies $(*)$.
Hence, it suffices to show that, if $f$ satisfies $(*)$, $f(m) = m$ for all $m \in \Z$, and $f(1/2) = 0$, then $f$ is the floor function.
Furthermore, plugging $b = 1$ into $(*)$ yields $f(x) + a = f(x + a)$ for all $x \in \mathbb{Q}$ and $a \in \Z$.
This means it suffices to show $f(x) = 0$ for all $x \in \mathbb{Q}$ with $0 \leq x < 1$.
Equivalently, it suffices to show that $f(a/b) = 0$ for any $a, b \in \N$ with $0 \leq a < b$.
The case $a = 0$ is trivial, so now we assume that $0 < a < b$.

Proceed by induction on $b \geq 2$.
We are done in the base case $b = 2$ since $f(1/2) = 0$.
Now fix some $b \geq 2$ and suppose that $f(a/b) = 0$ for all $0 < a < b$.
Then, for any $0 < a < b$, $(*)$ yields
$$ f\left(\frac{a}{b + 1}\right) = f\left(\frac{f(a/b) + a}{b + 1}\right) = f\left(\frac{a/b + a}{b + 1}\right) = f\left(\frac{a}{b}\right) = 0. $$
In particular, this also gives us $f\left(\frac{1}{b + 1}\right) = 0$.
Finally, for the case $a = b$, by $(*)$ and the previus equality, we have
$$ f\left(\frac{b}{b + 1}\right) = f\left(\frac{\frac{1}{b + 1} + (b - 1)}{b}\right) = f\left(\frac{b - 1}{b}\right) = 0. $$
Induction step is complete; we are done.
