\documentclass{article}

\usepackage{amsmath, amsfonts, amssymb, amsthm}
\usepackage{hyperref}

\setlength{\parindent}{0pt}
\setlength{\parskip}{5pt}

\newtheorem{lemma}{Lemma}

\title{IMO 2007 A3}
\author{}
\date{}

\begin{document}

\maketitle



\subsection*{Problem}

Let $F$ be a totally ordered field, and let $n$ be a positive integer.
Let $x, y \in F$ be positive elements such that $x^n + y^n = 1$.
Prove that
\[ \left(\sum_{k = 1}^n \frac{1 + x^{2k}}{1 + x^{4k}}\right) \left(\sum_{k = 1}^n \frac{1 + y^{2k}}{1 + y^{4k}}\right) < \frac{1}{(1 - x)(1 - y)}. \]



\subsection*{Solution}

Official solution: \url{https://www.imo-official.org/problems/IMO2007SL.pdf}

We just follow Solution 1 of the official solution.

The solution is based on the inequality $\dfrac{1 + t^2}{1 + t^4} < \dfrac{1}{t}$ for $t > 0$, $t \neq 1$.
This rearranges as $(t - 1)(t^3 - 1) = t^4 - t^3 - t + 1 > 0$.
Using this inequality, the left hand side is less than
\[ \left(\sum_{k = 1}^n \frac{1}{x^k}\right) \left(\sum_{k = 1}^n \frac{1}{y^k}\right) = \frac{x^{-n} - 1}{1 - x} \cdot \frac{y^{-n} - 1}{1 - y}. \]
Finally, we have $(x^{-n} - 1)(y^{-n} - 1) = 1$ since $x^n + y^n = 1$.
We are done.



\end{document}
