# IMO 2019 A1 (P1), Generalized Version

Let $G$ be an additive abelian group.
Fix an arbitrary function $g : G \to G$ with $g(0) = 0$.
Fix some $T \in End(G)$, and assume that $T$ is injective.
Determine all functions $f : G \to G$ such that, for all $x, y \in G$,
$$ f(g(x)) + Tf(y) = f(f(x + y)). $$



# Answer

Fix some $\phi \in End(G)$ and $C \in G$ such that $\phi \circ g = T \phi = \phi^2$ and $\phi(C) = U(C)$.
Then $x \mapsto \phi(x) + C$ satisfies the above equation.
Furthermore, all functions satisfying the above equation are of this form.

For the case $G = \Z$, note that the endomorphisms of $\Z$ are multiplications by some fixed integer.
Thus we can write $T = x \mapsto sx$ for some $s \neq 0$.
If $g \neq x \mapsto sx$, then $f = 0$ is the only solution.
If $g = x \mapsto sx$, then $f = 0$ and $f = x \mapsto sx + C$ for any integer $C$ are the solutions.

The original problem is a specialization with $g$ and $T$ being multiplication by $2$.
Thus the answer for that problem would be $f = 0$ and $f = x \mapsto 2x + C$ for any integer $C$.




# Solution

Official solution: <https://www.imo-official.org/problems/IMO2019SL.pdf>

We refer to Solution 2 and modify it for our generalization needs.
    
Let $f$ be an arbitrary function satisfying the above equation.
Let $C = f(0)$.
As in the official Solution 2, we get all the following:
$$ \forall x \in G, \quad f(f(x)) = Tf(x) + C, \tag{1} $$
$$ \forall x \in G, \quad f(g(x)) = T(f(x) - C) + C, \tag{2} $$
$$ \forall x, y \in G, \quad f(x + y) = f(x) + f(y) - C. \tag{3} $$
Conversely, one can check that $(1)$, $(2)$, and $(3)$ indeed implies the original equation.
Thus, it remains to classify all functions $f$ satisfying $(1)$, $(2)$, and $(3)$.

First notice that $(3)$ is equivalent to $f - C$ being additive.
In particular, $(3)$ means that we can write $f = \phi + C$ for some $\phi \in End(G)$.
Then $(2)$ reads as $\phi \circ g = T \phi$ and $(1)$ becomes
$$ \forall x \in G, \quad \phi(\phi(x) + C) = T \phi(x) + T(C) + C \to \phi^2(x) + \phi(C) = T \phi(x) + T(C). $$
Plugging in $x = 0$ yields $\phi(C) = T(C)$.
In turn, this implies that the above equation becomes $\phi^2 = T \phi$.
This shows that $\phi \circ g = T \phi = \phi^2$ and $\phi(C) = T(C)$.

## Case $G = \Z$

Now, consider the case where $G = \Z$.
Again, the endomorphisms of $\Z$ are multiplications by some fixed integer.
Thus, we can write $\phi(x) = kx$ and $T(x) = sx$ for some integer $k$ and $s$.
We have $s \neq 0$ since $T$ is injective.
The equation $T \phi = \phi^2$ implies $ks = k^2$, so either $m = s$ or $m = 0$.
The equation $\phi âˆ˜ g = T \phi$ reads as $k g(x) = skx$ for all integers $x$.
Thus, for $g \neq x \mapsto sx$, we have $k = 0$, and the equation $\phi(C) = T(C)$ reads as $sC = 0 \to C + 0$.
For $g = x \mapsto sx$ and $\phi(x) = sx$, any choice of $C$ works.
