\documentclass{article}

\usepackage{amsmath, amsfonts, amssymb, amsthm}
\usepackage{hyperref}

\setlength{\parindent}{0pt}
\setlength{\parskip}{5pt}

\title{IMO 2006 A2}
\author{}
\date{}

\begin{document}

\maketitle



\subsection*{Problem}

Let $F$ be a totally ordered field.
Define the sequence $(a_n)_{n \geq 0}$ in $F$ recursively by $a_0 = -1$ and, for all $n \geq 1$,
\[ \sum_{k = 0}^n \frac{a_k}{n - k + 1} = 0. \tag{*}\label{2006a2-eq0} \]
Prove that $a_n > 0$ for each $n \geq 1$.



\subsection*{Solution}

Official solution: \url{https://www.imo-official.org/problems/IMO2006SL.pdf}

The following solution is just a rewriting of the official solution.
The solution goes by strong induction.

\textit{\underline{Base case.}}
For the case $n = 1$,~\eqref{2006a2-eq0} implies $a_1 = \frac{1}{2} > 0$.

\textit{\underline{Induction step.}}
Fix some $n > 1$, and suppose that $a_k > 0$ for every $0 < k \leq n$.
Then,~\eqref{2006a2-eq0} yields
\begin{align*}
    0
    &= (n + 2) \sum_{k = 0}^{n + 1} \frac{a_k}{n - k + 2} - (n + 1) \sum_{k = 0}^n \frac{a_k}{n - k + 1} \\
    &= (n + 2) a_{n + 1} + \sum_{k = 0}^n a_k \left(\frac{n + 2}{n - k + 2} - \frac{n + 1}{n - k + 1}\right) \\
    &= (n + 2) a_{n + 1} - \sum_{k = 0}^n a_k \frac{k}{(n - k + 2)(n - k + 1)} \\
(n + 2) a_{n + 1}
    &= \sum_{k = 0}^n a_k \frac{k}{(n - k + 2)(n - k + 1)}.
\end{align*}
The term of the sum at $k = 0$ vanishes.
The rest of the terms are positive since $a_k > 0$ by induction hypothesis.
Excluding the term at $k = 0$, the sum is non-empty, so $(n + 2) a_{n + 1}$ is positive.
Induction step is complete.



\end{document}
